

$$77 \quad \lim_{x \rightarrow -1} \frac{x}{(x-1)^2} = \frac{-1}{(-1-1)^2} = \frac{-1}{4} = -\frac{1}{4}$$

$$78 \quad \lim_{x \rightarrow 2} \frac{x+2}{4-x} = \frac{2+2}{4-2} = \frac{4}{2} = 2$$

$$79 \quad \lim_{x \rightarrow +\infty} \frac{3}{x-2} = \frac{3}{+\infty-2} = \frac{3}{+\infty} = 0^+$$

$$80 \quad \lim_{x \rightarrow -\infty} \left(\frac{1}{2} + x\right)^2 = \left(\frac{1}{2} - \infty\right)^2 = (-\infty)^2 = +\infty$$

$$81 \quad \lim_{x \rightarrow +\infty} \frac{3}{(4-x)^4} = \frac{3}{(4-\infty)^4} = \frac{3}{(-\infty)^4} = \frac{3}{+\infty} = 0^+$$

$$82 \quad \lim_{x \rightarrow 4} \frac{x + \sqrt{x}}{2x - \sqrt{x}} = \frac{4 + \sqrt{4}}{2 \cdot 4 - \sqrt{4}} = \frac{4+2}{8-2} = \frac{6}{6} = 1$$